Update to using wordsTheory.

examples/Crypto/TWOFISH/twofishScript.sml
@@ -12,22 +12,13 @@ key schedule. For more information, please refer to
 
 (* For interactive work
   quietdec := true;
-  app load ["arithmeticTheory","metisLib","word8Lib","word32Lib"];
-  open arithmeticTheory word8Theory word32Theory 
-       pairTheory metisLib bitsTheory word8Lib;
+  app load ["arithmeticTheory","wordsLib"];
+  open arithmeticTheory wordsTheory pairTheory bitTheory wordsLib;
   quietdec := false;
 *)
 
 open HolKernel Parse boolLib bossLib
-     arithmeticTheory word8Theory word32Theory 
-     pairTheory metisLib bitsTheory word8Lib;
-
-(*---------------------------------------------------------------------------*)
-(* Make bindings to pre-existing stuff                                       *)
-(*---------------------------------------------------------------------------*)
-
-val RESTR_EVAL_TAC = computeLib.RESTR_EVAL_TAC;
-val ARW_TAC = RW_TAC arith_ss;
+     arithmeticTheory wordsTheory pairTheory bitTheory wordsLib;
 
 (*---------------------------------------------------------------------------*)
 (* Create the theory.                                                        *)
@@ -55,7 +46,6 @@ val _ = type_abbrev("keysched",
       word32 # word32 # word32 # word32 # word32 # word32 # word32 # word32 # 
       word32 # word32 # word32 # word32 # word32 # word32 # word32 # word32``);
 
-
 (*---------------------------------------------------------------------------*)
 (* Case analysis on a block and a pair of keys.                              *)
 (*---------------------------------------------------------------------------*)
@@ -74,119 +64,80 @@ val FORALL_KEY = Q.store_thm
 (* Operations on word8, word32 and word4.                                    *)
 (*---------------------------------------------------------------------------*)
 
-val W8_ROL_def = Define `W8_ROL (x:word8) n =  word8$word_ror x (word8$WL - n)`;
-val _ = overload_on ("#<<<",Term`$W8_ROL`);
-val _ = overload_on ("#>>>",Term`word8$word_ror`);  (* Word8_ROR *)
-val _ = set_fixity "#<<<" (Infixl 650);
-val _ = set_fixity "#>>>" (Infixl 650);
-val _ = overload_on ("##",Term`word8$bitwise_eor`);
-val _ = set_fixity "##" (Infixl 640);
-
-val W32_ROL_def = Define `W32_ROL (x:word32) n =  word32$word_ror x (word32$WL - n)`;
-val _ = overload_on ("<<<<",Term`$W32_ROL`)
-val _ = overload_on (">>>>",Term`word32$word_ror`);  (* Word32_ROR *)
-val _ = set_fixity "<<<<" (Infixl 630);
-val _ = set_fixity ">>>>" (Infixl 630);
-val _ = overload_on ("###",Term`word32$bitwise_eor`);
-val _ = set_fixity "###" (Infixl 620);
-
-
-val Word32_SHIFT_Inversion = Q.store_thm
-  ("Word32_SHIFT_Inversion",
-  `!s n. n < word32$WL ==> ((s >>>> n <<<< n = s) /\ (s <<<< n >>>> n = s))`,
-  REWRITE_TAC [W32_ROL_def,ROR_ADD] THEN ARW_TAC [SUB_LEFT_ADD] THEN
-  METIS_TAC [ROR_CYCLE, MULT_CLAUSES]);
-
-
 (* Word4 shifting operators *)
-val ROR4_def = Define `ROR4(x:word8, n) = (x >> n) & ((x << (4 - n)) & 0xffffw)`;
-val ROL4_def = Define `ROR4(x:word8, n) = (x << n) & ((x >> (4 - n)) & 0xffffw)`;
+val ROR4_def = Define`ROR4(x:word8, n) = x >> n && x << (4 - n)`;
+val ROL4_def = Define`ROL4(x:word8, n) = x << n && x >> (4 - n)`;
 
+val _ = wordsLib.guess_lengths();
 
 (* Conversion between word8*word8*word8*word8 and word32 *)
-val toLarge_def = Define `toLarge (a3:word8,a2:word8,a1:word8,a0:word8) = 
-	word32$n2w(w2n(a3)) << 24 + word32$n2w(w2n(a2)) << 16 + 
-	word32$n2w(w2n(a1)) << 8 + word32$n2w(w2n(a0)) : word32`;
-val fromLarge_def = Define `fromLarge (a:word32) = (word8$n2w(w2n(a >> 24)), 
-	word8$n2w(w2n((a >> 16) & 0xffw)), word8$n2w(w2n((a >> 8) & 0xffw)),
-	word8$n2w(w2n(a & 0xffw))) : word8 # word8 # word8 # word8 `;
 
+val toLarge_def = Define`toLarge (a3:word8,a2:word8,a1:word8,a0:word8) = 
+   a3 @@ a2 @@ a1 @@ a0`;
+
+val fromLarge_def = Define`fromLarge (a:word32) =
+   ((31 >< 24) a, (23 >< 16) a, (15 >< 8) a, (7 >< 0) a)`;
 
 (*---------------------------------------------------------------------------*)
 (* Multiply a byte representing a polynomial by x. 			     *)
 (*---------------------------------------------------------------------------*)
 
 (* For MDS multiplication, v(x) = x^8 + x^6 + x^5 + x^3 + 1 , i.e. 0wx165    *)
+
 val xtime1_def = Define
   `xtime1 (w : word8) =
-     if MSB w then w << 1 ## 0x165w
-              else w << 1`;
+     if word_msb w then w << 1 ?? 0x165w else w << 1`;
 
 val _ = set_fixity "**" (Infixl 675);
 
-val (Mult1_def,Mult1_ind) =
- Defn.tprove
-  (Hol_defn "Mult1"
-     `b1 ** b2 =
-        if b1 = 0w then 0w else
-        if LSB b1
-           then b2 # ((word8$word_lsr b1 1) ** xtime1 b2)
-           else      (word8$word_lsr b1 1) ** xtime1 b2`,
-   WF_REL_TAC `measure (word8$w2n o FST)` THEN
-   STRIP_TAC THEN word8CasesLib.word8Cases_on `b1` THEN
-   RW_TAC std_ss [] THEN REPEAT (POP_ASSUM MP_TAC) THEN WORD_TAC);
-
-val _ = save_thm("Mult1_def",Mult1_def);
-val _ = save_thm("Mult1_ind",Mult1_ind);
+val Mult1_def = xDefine "Mult1"
+  `b1 ** b2 =
+     if b1 = 0w :word8 then 0w else
+     if word_lsb b1
+        then b2 ?? ((b1 >>> 1) ** xtime1 b2)
+        else        (b1 >>> 1) ** xtime1 b2`;
 
 (* For RS multiplication, v(x) = x^8 + x^6 + x^3 + x^2 + 1 , i.e. 0wx14D*)
+
 val xtime2_def = Define
   `xtime2 (w : word8) =
-     if MSB w then w << 1 ## 0x14Dw
-     else w << 1`;
+     if word_msb w then w << 1 ?? 0x14Dw else w << 1`;
 
 val _ = set_fixity "***" (Infixl 675);
 
-val (Mult2_def,Mult2_ind) =
- Defn.tprove
-  (Hol_defn "Mult2"
-     `b1 *** b2 =
-        if b1 = 0w then 0w else
-        if LSB b1
-           then b2 # ((word8$word_lsr b1 1) *** xtime2 b2)
-           else      (word8$word_lsr b1 1) *** xtime2 b2`,
-   WF_REL_TAC `measure (word8$w2n o FST)` THEN
-   STRIP_TAC THEN word8CasesLib.word8Cases_on `b1` THEN
-   RW_TAC std_ss [] THEN REPEAT (POP_ASSUM MP_TAC) THEN WORD_TAC);
+val Mult2_def = xDefine "Mult2"
+  `b1 *** b2 =
+     if b1 = 0w :word8 then 0w else
+     if word_lsb b1
+        then b2 ?? ((b1 >>> 1) *** xtime2 b2)
+        else        (b1 >>> 1) *** xtime2 b2`;
 
-val _ = save_thm("Mult2_def",Mult2_def);
-val _ = save_thm("Mult2_ind",Mult2_ind);
+(*---------------------------------------------------------------------------*)
+(* Matrix Column Multiplication                                              *)
+(*---------------------------------------------------------------------------*)
 
-(*-------------------------------------------------------------------------------*)
-(* Matrix Column Multiplication 						 *)
-(*-------------------------------------------------------------------------------*)
-
-val InvW_def = Define `
+val InvW_def = Define`
     InvW (m0,m1,m2,m3): (word8 # word8 # word8 # word8) = (m3,m2,m1,m0)`;
 
 (* Multiply the MDS matrix *)
-val MDSMul_def = Define `MDSMul(m0,m1,m2,m3) =
-  ((0x01w ** m0) ## (0xEFw ** m1) ## (0x5Bw ** m2) ## (0x5Bw ** m3),
-   (0x5Bw ** m0) ## (0xEFw ** m1) ## (0xEFw ** m2) ## (0x01w ** m3),
-   (0xEFw ** m0) ## (0x5Bw ** m1) ## (0x01w ** m2) ## (0xEFw ** m3),
-   (0xEFw ** m0) ## (0x01w ** m1) ## (0xEFw ** m2) ## (0x5Bw ** m3))`;
+
+val MDSMul_def = Define`MDSMul(m0,m1,m2,m3) =
+  ((0x01w ** m0) ?? (0xEFw ** m1) ?? (0x5Bw ** m2) ?? (0x5Bw ** m3),
+   (0x5Bw ** m0) ?? (0xEFw ** m1) ?? (0xEFw ** m2) ?? (0x01w ** m3),
+   (0xEFw ** m0) ?? (0x5Bw ** m1) ?? (0x01w ** m2) ?? (0xEFw ** m3),
+   (0xEFw ** m0) ?? (0x01w ** m1) ?? (0xEFw ** m2) ?? (0x5Bw ** m3))`;
 
 (* Multiply the RS matrix *)
-val RSMul_def = Define `RSMul(m0,m1,m2,m3,m4,m5,m6,m7) =
-  ((0x01w *** m0) ## (0xA4w *** m1) ## (0x55w *** m2) ## (0x87w *** m3) ##
-   (0x5Aw *** m4) ## (0x58w *** m5) ## (0xDBw *** m6) ## (0x9Ew *** m7),
-   (0xA4w *** m0) ## (0x56w *** m1) ## (0x82w *** m2) ## (0xF3w *** m3) ##
-   (0x1Ew *** m4) ## (0xC6w *** m5) ## (0x68w *** m6) ## (0xE5w *** m7),
-   (0x02w *** m0) ## (0xA1w *** m1) ## (0xFCw *** m2) ## (0xC1w *** m3) ##
-   (0x47w *** m4) ## (0xAEw *** m5) ## (0x3Dw *** m6) ## (0x19w *** m7),
-   (0xA4w *** m0) ## (0x55w *** m1) ## (0x87w *** m2) ## (0x5Aw *** m3) ##
-   (0x58w *** m4) ## (0xDBw *** m5) ## (0x9Ew *** m6) ## (0x03w *** m7))`;
 
+val RSMul_def = Define`RSMul(m0,m1,m2,m3,m4,m5,m6,m7) =
+  ((0x01w *** m0) ?? (0xA4w *** m1) ?? (0x55w *** m2) ?? (0x87w *** m3) ??
+   (0x5Aw *** m4) ?? (0x58w *** m5) ?? (0xDBw *** m6) ?? (0x9Ew *** m7),
+   (0xA4w *** m0) ?? (0x56w *** m1) ?? (0x82w *** m2) ?? (0xF3w *** m3) ??
+   (0x1Ew *** m4) ?? (0xC6w *** m5) ?? (0x68w *** m6) ?? (0xE5w *** m7),
+   (0x02w *** m0) ?? (0xA1w *** m1) ?? (0xFCw *** m2) ?? (0xC1w *** m3) ??
+   (0x47w *** m4) ?? (0xAEw *** m5) ?? (0x3Dw *** m6) ?? (0x19w *** m7),
+   (0xA4w *** m0) ?? (0x55w *** m1) ?? (0x87w *** m2) ?? (0x5Aw *** m3) ??
+   (0x58w *** m4) ?? (0xDBw *** m5) ?? (0x9Ew *** m6) ?? (0x03w *** m7))`;
 
 (*---------------------------------------------------------------------------*)
 (* The permutations q0 and q1 are fixed permutations on 8-bit values.	     *)
@@ -194,7 +145,8 @@ val RSMul_def = Define `RSMul(m0,m1,m2,m3,m4,m5,m6,m7) =
 (*---------------------------------------------------------------------------*)
 
 (* The 4-bit S-boxes For the permutation q0 *)
-val t00_def = Define ` 
+
+val t00_def = Define` 
   t00 (x:word8) = 
     case x of 
     0w -> 0x8w || 1w -> 0x1w || 2w -> 0x7w || 3w -> 0xDw ||
@@ -202,7 +154,7 @@ val t00_def = Define `
     8w -> 0x0w || 9w -> 0xBw || 10w -> 0x5w || 11w -> 0x9w ||
     12w -> 0xEw || 13w -> 0xCw || 14w -> 0xAw || 15w -> 0x4w : word8`;
 
-val t01_def = Define `
+val t01_def = Define`
   t01 (x:word8) =
     case x of
     0w -> 0xEw || 1w -> 0xCw || 2w -> 0xBw || 3w -> 0x8w ||
@@ -210,7 +162,7 @@ val t01_def = Define `
     8w -> 0xFw || 9w -> 0x4w || 10w -> 0xAw || 11w -> 0x6w ||
     12w -> 0x7w || 13w -> 0x0w || 14w -> 0x9w || 15w -> 0xDw : word8`;
 
-val t02_def = Define `
+val t02_def = Define`
   t02 (x:word8) =
     case x of
     0w -> 0xBw || 1w -> 0xAw || 2w -> 0x5w || 3w -> 0xEw ||
@@ -218,7 +170,7 @@ val t02_def = Define `
     8w -> 0xCw || 9w -> 0x8w || 10w -> 0xFw || 11w -> 0x3w ||
     12w -> 0x2w || 13w -> 0x4w || 14w -> 0x7w || 15w -> 0x1w : word8`;
 
-val t03_def = Define `
+val t03_def = Define`
   t03 (x:word8) =
     case x of
     0w -> 0xDw || 1w -> 0x7w || 2w -> 0xFw || 3w -> 0x4w ||
@@ -226,9 +178,9 @@ val t03_def = Define `
     8w -> 0x9w || 9w -> 0xBw || 10w -> 0x3w || 11w -> 0x0w ||
     12w -> 0x8w || 13w -> 0x5w || 14w -> 0xCw || 15w -> 0xAw : word8`;
 
-
 (* The 4-bit S-boxes For the permutation q1 *)
-val t10_def = Define `
+
+val t10_def = Define`
   t10 (x:word8) =
     case x of
     0w -> 0x2w || 1w -> 0x8w || 2w -> 0xBw || 3w -> 0xDw ||
@@ -236,7 +188,7 @@ val t10_def = Define `
     8w -> 0x3w || 9w -> 0x1w || 10w -> 0x9w || 11w -> 0x4w ||
     12w -> 0x0w || 13w -> 0xAw || 14w -> 0xCw || 15w -> 0x5w : word8`;
 
-val t11_def = Define `
+val t11_def = Define`
   t11 (x:word8) =
     case x of
     0w -> 0x1w || 1w -> 0xEw || 2w -> 0x2w || 3w -> 0xBw ||
@@ -244,7 +196,7 @@ val t11_def = Define `
     8w -> 0x6w || 9w -> 0xDw || 10w -> 0xAw || 11w -> 0x5w ||
     12w -> 0xFw || 13w -> 0x9w || 14w -> 0x0w || 15w -> 0x8w : word8`;
 
-val t12_def = Define `
+val t12_def = Define`
   t12 (x:word8) =
     case x of
     0w -> 0x4w || 1w -> 0xCw || 2w -> 0x7w || 3w -> 0x5w ||
@@ -252,7 +204,7 @@ val t12_def = Define `
     8w -> 0x0w || 9w -> 0xEw || 10w -> 0xDw || 11w -> 0x8w ||
     12w -> 0x2w || 13w -> 0xBw || 14w -> 0x3w || 15w -> 0xFw : word8`;
 
-val t13_def = Define `
+val t13_def = Define`
   t13 (x:word8) =
     case x of
     0w -> 0xBw || 1w -> 0x9w || 2w -> 0x5w || 3w -> 0x1w ||
@@ -260,257 +212,294 @@ val t13_def = Define `
     8w -> 0x6w || 9w -> 0x4w || 10w -> 0x7w || 11w -> 0xFw ||
     12w -> 0x2w || 13w -> 0x0w || 14w -> 0x8w || 15w -> 0xAw : word8`;
 
+(* First, the byte is split into two nibbles. These are combined in a        *)
+(* bijective mixing step. Each nibble is then passed through its own 4-bit   *)
+(* fixed S-box. This is followed by another mixing step and S-box lookup.    *)
+(* Finally, the two nibbles are recombined into a byte.                      *)
 
-(*  First, the byte is split into two nibbles. These are combined in a bijective mixing   *)
-(*  step. Each nibble is then passed through its own 4-bit fixed S-box. This is followed  *)
-(*  by another mixing step and S-box lookup. Finally, the two nibbles are recombined into *)
-(*  a byte. 										  *)
-val qq_def = Define `
+val qq_def = Define`
   qq t0 t1 t2 t3 (x:word8) =
-    let (a0, b0) = ((x >> 4) & 0xfw, x & 0xfw) in
-    let (a1, b1) = (a0 ## b0, a0 ## ROR4(b0,1) ## (8w*a0 & 0xfw)) in
+    let (a0, b0) = ((x >> 4) && 0xfw, x && 0xfw) in
+    let (a1, b1) = (a0 ?? b0, a0 ?? ROR4(b0,1) ?? (8w*a0 && 0xfw)) in
     let (a2, b2) = (t0(a1), t1(b1)) in
-    let (a3, b3) = (a2 ## a2, a0 ## ROR4(b2,1) ## (8w*a2 & 0xfw)) in
+    let (a3, b3) = (a2 ?? a2, a0 ?? ROR4(b2,1) ?? (8w*a2 && 0xfw)) in
     let (a4, b4) = (t2(a3), t3(b3))
     in 16w * b4 + a4 : word8`;
 
-val q0_def = Define `q0 = qq t00 t01 t02 t03`;
-val q1_def = Define `q1 = qq t10 t11 t12 t13`;
+val q0_def = Define`q0 = qq t00 t01 t02 t03`;
+val q1_def = Define`q1 = qq t10 t11 t12 t13`;
 
-(*----------------------------------------------------------------------------------------*)
-(* Function h takes two inputs--a 32-bit word X and a list L = (L0,...,Lk ) (here k = 4)  *)
-(* of 32-bit words of and produces one word of output. This function works in k stages.   *)
-(* In each stage, the four bytes are each passed through a fixed S-box, and               *)
-(* xored with a byte derived from the list. Finally, the bytes are once again passed      *)
-(* through a fixed Sbox, and the four bytes are multiplied by the MDS matrix.             *)
-(*----------------------------------------------------------------------------------------*)
+(*---------------------------------------------------------------------------*)
+(* Function h takes two inputs--a 32-bit word X and a list L = (L0,...,Lk )  *)
+(* (here k = 4) of 32-bit words of and produces one word of output. This     *)
+(* function works in k stages. In each stage, the four bytes are each        *)
+(* passed through a fixed S-box, and xored with a byte derived from the list.*)
+(* Finally, the bytes are once again passed through a fixed Sbox, and the    *)
+(* four bytes are multiplied by the MDS matrix.                              *)
+(*---------------------------------------------------------------------------*)
 
-val fun_h_def = Define `
-  fun_h((x3,x2,x1,x0), ((l33,l32,l31,l30),(l23,l22,l21,l20),(l13,l12,l11,l10),(l03,l02,l01,l00)))
-  = let (y0,y1,y2,y3) = (x0,x1,x2,x3) in
-    let (y0,y1,y2,y3) = (q1(y0) ## l30, q0(y1) ## l31, q0(y2) ## l32, q1(y3) ## l33) in (* k=4 *)
-    let (y0,y1,y2,y3) = (q1(y0) ## l20, q1(y1) ## l21, q0(y2) ## l22, q0(y3) ## l23) in (* k=3 *)
-    let (y0,y1,y2,y3) = (q1(q0(q0(y0) ## l10) ## l00), q0(q0(q1(y1) ## l11) ## l01),
-                         q1(q1(q0(y2) ## l12) ## l02), q0(q1(q1(y3) ## l13) ## l03)) in (* k=2 *)
-    let (y0,y1,y2,y3) = (q1(q0(q0(y0) ## l10) ## l00), q0(q0(q1(y1) ## l11) ## l01),
-                         q1(q1(q0(y2) ## l12) ## l02), q0(q1(q1(y3) ## l13) ## l03))    (* k=1 *)
-    in InvW(MDSMul(y0,y1,y2,y3))`;
+val fun_h_def = Define`
+  fun_h
+   ((x3,x2,x1,x0),(l33,l32,l31,l30),(l23,l22,l21,l20),
+    (l13,l12,l11,l10),l03,l02,l01,l00) =
+ (let (y0,y1,y2,y3) = (x0,x1,x2,x3) in
+  let (y0,y1,y2,y3) =
+        (q1 y0 ?? l30,q0 y1 ?? l31,q0 y2 ?? l32,q1 y3 ?? l33)          (* k=4 *)
+  in
+  let (y0,y1,y2,y3) =
+        (q1 y0 ?? l20,q1 y1 ?? l21,q0 y2 ?? l22,q0 y3 ?? l23)          (* k=3 *)
+  in
+  let (y0,y1,y2,y3) =
+        (q1 (q0 (q0 y0 ?? l10) ?? l00), q0 (q0 (q1 y1 ?? l11) ?? l01),
+         q1 (q1 (q0 y2 ?? l12) ?? l02), q0 (q1 (q1 y3 ?? l13) ?? l03)) (* k=2 *)
+  in
+  let (y0,y1,y2,y3) =
+        (q1 (q0 (q0 y0 ?? l10) ?? l00), q0 (q0 (q1 y1 ?? l11) ?? l01),
+         q1 (q1 (q0 y2 ?? l12) ?? l02), q0 (q1 (q1 y3 ?? l13) ?? l03)) (* k=1 *)
+  in
+    InvW (MDSMul (y0,y1,y2,y3)))`;
 
-(*----------------------------------------------------------------------------------------*)
-(* Take the key bytes in groups of 8, interpreting them as a vector over                  *)
-(* GF(2^8), and multiplying them by a 4bytes 8 matrix derived from an RS code.            *)
-(*----------------------------------------------------------------------------------------*)
+(*---------------------------------------------------------------------------*)
+(* Take the key bytes in groups of 8, interpreting them as a vector over     *)
+(* GF(2^8), and multiplying them by a 4bytes 8 matrix derived from an RS code.*)
+(*---------------------------------------------------------------------------*)
 
-val genM_def = Define `
-  genM ((m31,m30,m29,m28,m27,m26,m25,m24,m23,m22,m21,m20,m19,m18,m17,m16,m15,
-        m14,m13,m12,m11,m10,m9,m8,m7,m6,m5,m4,m3,m2,m1,m0):initkeys)
-  =  let Me = ((m3,m2,m1,m0),(m11,m10,m9,m8),(m19,m18,m17,m16),(m27,m26,m25,m24)) in
-     let Mo = ((m7,m6,m5,m4),(m15,m14,m13,m12),(m23,m22,m21,m20),(m31,m30,m29,m28))
-     in (Me, Mo)`;
+val genM_def = Define`
+  genM
+    ((m31,m30,m29,m28,m27,m26,m25,m24,m23,m22,m21,m20,m19,m18,m17,m16,m15,
+      m14,m13,m12,m11,m10,m9,m8,m7,m6,m5,m4,m3,m2,m1,m0):initkeys) =
+  let Me = ((m3,m2,m1,m0),(m11,m10,m9,m8),(m19,m18,m17,m16),(m27,m26,m25,m24))
+  in
+  let Mo = ((m7,m6,m5,m4),(m15,m14,m13,m12),(m23,m22,m21,m20),(m31,m30,m29,m28))
+  in
+    (Me, Mo)`;
 
-val genS_def = Define `
-  genS ((m31,m30,m29,m28,m27,m26,m25,m24,m23,m22,m21,m20,m19,m18,m17,m16,m15,
-        m14,m13,m12,m11,m10,m9,m8,m7,m6,m5,m4,m3,m2,m1,m0):initkeys)
-  =
-     (InvW(RSMul(m24,m25,m26,m27,m28,m29,m30,m31)), InvW(RSMul(m16,m17,m18,m19,m20,m21,m22,m23)),
-      InvW(RSMul(m8,m9,m10,m11,m12,m13,m14,m15)), InvW(RSMul(m0,m1,m2,m3,m4,m5,m6,m7)))`;
+val genS_def = Define`
+  genS
+    (m31,m30,m29,m28,m27,m26,m25,m24,m23,m22,m21,m20,m19,m18,m17,m16,
+     m15,m14,m13,m12,m11,m10,m9,m8,m7,m6,m5,m4,m3,m2,m1,m0) =
+  (InvW (RSMul (m24,m25,m26,m27,m28,m29,m30,m31)),
+   InvW (RSMul (m16,m17,m18,m19,m20,m21,m22,m23)),
+   InvW (RSMul (m8,m9,m10,m11,m12,m13,m14,m15)),
+   InvW (RSMul (m0,m1,m2,m3,m4,m5,m6,m7)))`;
 
-(*----------------------------------------------------------------------------------------*)
-(* The words of the expanded key are defined using the h function. For Ai the byte values *)
-(* are 2i, and the second argument of h is Me. Bi is computed similarly using 2i + 1 as   *)
-(* the byte value and Mo as the second argument, with an extra rotate over 8 bits.        *)
-(* The values Ai and Bi are combined in a PHT. One of the results is further              *)
-(* rotated by 9 bits.                                                                     *)
-(*----------------------------------------------------------------------------------------*)
+(*---------------------------------------------------------------------------*)
+(* The words of the expanded key are defined using the h function. For Ai    *)
+(* the byte values are 2i, and the second argument of h is Me. Bi is         *)
+(* computed similarly using 2i + 1 as the byte value and Mo as the second    *)
+(* argument, with an extra rotate over 8 bits.  The values Ai and Bi are     *)
+(* combined in a PHT. One of the results is further rotated by 9 bits.       *)
+(*---------------------------------------------------------------------------*)
 
-val e_rnd_def = Define `
+val e_rnd_def = Define`
   e_rnd(Me,Mo,i) =
-    let i = word8$n2w i in
+    let i = n2w i in
     let Ai = toLarge(fun_h((2w*i, 2w*i, 2w*i, 2w*i), Me)) in
-    let Bi = toLarge(fun_h((2w*i+1w, 2w*i+1w, 2w*i+1w, 2w*i+1w), Mo)) <<<< 8 in
-    let K2i = word32$bitwise_and (Ai + Bi) 0xffffffffw in
-    let K2i_1 = (word32$bitwise_and (Ai + 2w * Bi) 0xffffffffw) <<<< 9
+    let Bi = toLarge(fun_h((2w*i+1w, 2w*i+1w, 2w*i+1w, 2w*i+1w), Mo)) #<< 8 in
+    let K2i = (Ai + Bi) && 0xffffffffw in
+    let K2i_1 = ((Ai + 2w * Bi) && 0xffffffffw) #<< 9
     in (K2i, K2i_1)`;
 
-val expandKeys_def = Define `
-  expandKeys(Me,Mo) = (
-    FST(e_rnd(Me,Mo,0)), SND(e_rnd(Me,Mo,0)), FST(e_rnd(Me,Mo,1)), SND(e_rnd(Me,Mo,1)),
-    FST(e_rnd(Me,Mo,2)), SND(e_rnd(Me,Mo,2)), FST(e_rnd(Me,Mo,3)), SND(e_rnd(Me,Mo,3)),
-    FST(e_rnd(Me,Mo,4)), SND(e_rnd(Me,Mo,4)), FST(e_rnd(Me,Mo,5)), SND(e_rnd(Me,Mo,5)),
-    FST(e_rnd(Me,Mo,6)), SND(e_rnd(Me,Mo,6)), FST(e_rnd(Me,Mo,7)), SND(e_rnd(Me,Mo,7)),
-    FST(e_rnd(Me,Mo,8)), SND(e_rnd(Me,Mo,8)), FST(e_rnd(Me,Mo,9)), SND(e_rnd(Me,Mo,9)),
-    FST(e_rnd(Me,Mo,10)), SND(e_rnd(Me,Mo,10)),FST(e_rnd(Me,Mo,11)), SND(e_rnd(Me,Mo,11)),
-    FST(e_rnd(Me,Mo,12)), SND(e_rnd(Me,Mo,12)), FST(e_rnd(Me,Mo,13)), SND(e_rnd(Me,Mo,13)),
-    FST(e_rnd(Me,Mo,14)), SND(e_rnd(Me,Mo,14)), FST(e_rnd(Me,Mo,15)), SND(e_rnd(Me,Mo,15)),
-    FST(e_rnd(Me,Mo,16)), SND(e_rnd(Me,Mo,16)), FST(e_rnd(Me,Mo,17)), SND(e_rnd(Me,Mo,17)),
-    FST(e_rnd(Me,Mo,18)), SND(e_rnd(Me,Mo,18)), FST(e_rnd(Me,Mo,19)), SND(e_rnd(Me,Mo,19)))`;
+val expandKeys_def = Define`
+  expandKeys (Me,Mo) =
+     (FST (e_rnd (Me,Mo,0)),SND (e_rnd (Me,Mo,0)),
+      FST (e_rnd (Me,Mo,1)),SND (e_rnd (Me,Mo,1)),
+      FST (e_rnd (Me,Mo,2)),SND (e_rnd (Me,Mo,2)),
+      FST (e_rnd (Me,Mo,3)),SND (e_rnd (Me,Mo,3)),
+      FST (e_rnd (Me,Mo,4)),SND (e_rnd (Me,Mo,4)),
+      FST (e_rnd (Me,Mo,5)),SND (e_rnd (Me,Mo,5)),
+      FST (e_rnd (Me,Mo,6)),SND (e_rnd (Me,Mo,6)),
+      FST (e_rnd (Me,Mo,7)),SND (e_rnd (Me,Mo,7)),
+      FST (e_rnd (Me,Mo,8)),SND (e_rnd (Me,Mo,8)),
+      FST (e_rnd (Me,Mo,9)),SND (e_rnd (Me,Mo,9)),
+      FST (e_rnd (Me,Mo,10)),SND (e_rnd (Me,Mo,10)),
+      FST (e_rnd (Me,Mo,11)),SND (e_rnd (Me,Mo,11)),
+      FST (e_rnd (Me,Mo,12)),SND (e_rnd (Me,Mo,12)),
+      FST (e_rnd (Me,Mo,13)),SND (e_rnd (Me,Mo,13)),
+      FST (e_rnd (Me,Mo,14)),SND (e_rnd (Me,Mo,14)),
+      FST (e_rnd (Me,Mo,15)),SND (e_rnd (Me,Mo,15)),
+      FST (e_rnd (Me,Mo,16)),SND (e_rnd (Me,Mo,16)),
+      FST (e_rnd (Me,Mo,17)),SND (e_rnd (Me,Mo,17)),
+      FST (e_rnd (Me,Mo,18)),SND (e_rnd (Me,Mo,18)),
+      FST (e_rnd (Me,Mo,19)),SND (e_rnd (Me,Mo,19)))`;
 
-(*----------------------------------------------------------------------------------------*)
-(*----------------------------------------------------------------------------------------*)
+(*---------------------------------------------------------------------------*)
+(*---------------------------------------------------------------------------*)
 
-val ROTKEYS_def = Define `
-  ROTKEYS ((k0,k1,k2,k3,k4,k5,k6,k7,k8,k9,k10,k11,k12,k13,k14,k15,k16,k17,k18,k19,
-        k20,k21,k22,k23,k24,k25,k26,k27,k28,k29,k30,k31,k32,k33,k34,k35,k36,k37,k38,k39):keysched)
-  =  (k2,k3,k4,k5,k6,k7,k8,k9,k10,k11,k12,k13,k14,k15,k16,k17,k18,k19,
-      k20,k21,k22,k23,k24,k25,k26,k27,k28,k29,k30,k31,k32,k33,k34,k35,k36,k37,k38,k39,k0,k1)`;
+val ROTKEYS_def = Define`
+  ROTKEYS
+   (k0,k1,k2,k3,k4,k5,k6,k7,k8,k9,k10,k11,k12,k13,k14,k15,k16,k17,
+    k18,k19,k20,k21,k22,k23,k24,k25,k26,k27,k28,k29,k30,k31,k32,k33,
+    k34,k35,k36,k37,k38,k39) =
+ (k2,k3,k4,k5,k6,k7,k8,k9,k10,k11,k12,k13,k14,k15,k16,k17,k18,k19,
+  k20,k21,k22,k23,k24,k25,k26,k27,k28,k29,k30,k31,k32,k33,k34,k35,
+  k36,k37,k38,k39,k0,k1)`;
 
-val ROTKEYS8_def = Define `
-  ROTKEYS8 ((k0,k1,k2,k3,k4,k5,k6,k7,k8,k9,k10,k11,k12,k13,k14,k15,k16,k17,k18,k19,
-        k20,k21,k22,k23,k24,k25,k26,k27,k28,k29,k30,k31,k32,k33,k34,k35,k36,k37,k38,k39):keysched)
-  =  (k8,k9,k10,k11,k12,k13,k14,k15,k16,k17,k18,k19,k20,k21,k22,k23,k24,k25,k26,k27,k28,
-        k29,k30,k31,k32,k33,k34,k35,k36,k37,k38,k39,k0,k1,k2,k3,k4,k5,k6,k7)`;
+val ROTKEYS8_def = Define`
+  ROTKEYS8
+   (k0,k1,k2,k3,k4,k5,k6,k7,k8,k9,k10,k11,k12,k13,k14,k15,k16,k17,
+    k18,k19,k20,k21,k22,k23,k24,k25,k26,k27,k28,k29,k30,k31,k32,k33,
+    k34,k35,k36,k37,k38,k39) =
+ (k8,k9,k10,k11,k12,k13,k14,k15,k16,k17,k18,k19,k20,k21,k22,k23,k24,
+  k25,k26,k27,k28,k29,k30,k31,k32,k33,k34,k35,k36,k37,k38,k39,k0,k1,
+  k2,k3,k4,k5,k6,k7)`;
 
-val GETKEYS_def = Define `
-  GETKEYS ((k0,k1,k2,k3,k4,k5,k6,k7,k8,k9,k10,k11,k12,k13,k14,k15,k16,k17,k18,k19,
-        k20,k21,k22,k23,k24,k25,k26,k27,k28,k29,k30,k31,k32,k33,k34,k35,k36,k37,k38,k39):keysched)
-  =  (k0,k1)`;
+val GETKEYS_def = Define`
+  GETKEYS
+   (k0,k1,k2,k3,k4,k5,k6,k7,k8,k9,k10,k11,k12,k13,k14,k15,k16,k17,
+    k18,k19,k20,k21,k22,k23,k24,k25,k26,k27,k28,k29,k30,k31,k32,k33,
+    k34,k35,k36,k37,k38,k39) =
+ (k0,k1)`;
 
-val FORALL_INITKEYS = Q.prove
-(`(!x:initkeys. P x) = !k0 k1 k2 k3 k4 k5 k6 k7 k8 k9 k10 k11 k12 k13 k14 k15 k16 
-	k17 k18 k19 k20 k21 k22 k23 k24 k25 k26 k27 k28 k29 k30 k31.
-        P(k0,k1,k2,k3,k4,k5,k6,k7,k8,k9,k10,k11,k12,k13,k14,k15,k16,k17,k18,k19,k20,
-          k21,k22,k23,k24,k25,k26,k27,k28,k29,k30,k31)`,
+val FORALL_INITKEYS = Q.prove(
+ `(!x:initkeys. P x) =
+   !k0 k1 k2 k3 k4 k5 k6 k7 k8 k9 k10 k11 k12 k13 k14 k15 k16 k17 k18
+      k19 k20 k21 k22 k23 k24 k25 k26 k27 k28 k29 k30 k31.
+    P (k0,k1,k2,k3,k4,k5,k6,k7,k8,k9,k10,k11,k12,k13,k14,k15,k16,k17,
+       k18,k19,k20,k21,k22,k23,k24,k25,k26,k27,k28,k29,k30,k31)`,
   SIMP_TAC std_ss [FORALL_PROD]);
 
-val FORALL_KEYSCHEDS = Q.prove
-(`(!x:keysched. P x) = !k0 k1 k2 k3 k4 k5 k6 k7 k8 k9 k10 k11 k12 k13 k14 k15 k16 k17 k18 k19 k20
-             k21 k22 k23 k24 k25 k26 k27 k28 k29 k30 k31 k32 k33 k34 k35 k36 k37 k38 k39.
-             P(k0,k1,k2,k3,k4,k5,k6,k7,k8,k9,k10,k11,k12,k13,k14,k15,k16,k17,k18,k19,k20,
-             k21,k22,k23,k24,k25,k26,k27,k28,k29,k30,k31,k32,k33,k34,k35,k36,k37,k38,k39)`,
+val FORALL_KEYSCHEDS = Q.prove(
+ `(!x:keysched. P x) =
+  !k0 k1 k2 k3 k4 k5 k6 k7 k8 k9 k10 k11 k12 k13 k14 k15 k16 k17 k18
+     k19 k20 k21 k22 k23 k24 k25 k26 k27 k28 k29 k30 k31 k32 k33 k34
+     k35 k36 k37 k38 k39.
+   P (k0,k1,k2,k3,k4,k5,k6,k7,k8,k9,k10,k11,k12,k13,k14,k15,k16,k17,
+      k18,k19,k20,k21,k22,k23,k24,k25,k26,k27,k28,k29,k30,k31,k32,k33,
+      k34,k35,k36,k37,k38,k39)`,
   SIMP_TAC std_ss [FORALL_PROD]);
 
 (*---------------------------------------------------------------------------*)
 (* Sanity check                                                              *)
 (*---------------------------------------------------------------------------*)
 
-val toList_def = Define `
+val toList_def = Define`
   toList (k:keysched) = 
-   let (k0,k1,k2,k3,k4,k5,k6,k7,k8,k9,k10,k11,k12,k13,k14,k15,k16,k17,k18,k19,
-        k20,k21,k22,k23,k24,k25,k26,k27,k28,k29,k30,k31,k32,k33,k34,k35,k36,k37,k38,k39) = k in
-     [k0;k1;k2;k3;k4;k5;k6;k7;k8;k9;k10;k11;k12;k13;k14;k15;k16;k17;k18;k19;
-      k20;k21;k22;k23;k24;k25;k26;k27;k28;k29;k30;k31;k32;k33;k34;k35;k36;k37;k38;k39]`;
+  (let (k0,k1,k2,k3,k4,k5,k6,k7,k8,k9,k10,k11,k12,k13,k14,k15,k16,
+        k17,k18,k19,k20,k21,k22,k23,k24,k25,k26,k27,k28,k29,k30,k31,
+        k32,k33,k34,k35,k36,k37,k38,k39) = k
+   in
+     [k0; k1; k2; k3; k4; k5; k6; k7; k8; k9; k10; k11; k12; k13;
+      k14; k15; k16; k17; k18; k19; k20; k21; k22; k23; k24; k25;
+      k26; k27; k28; k29; k30; k31; k32; k33; k34; k35; k36; k37;
+      k38; k39])`;
 
-val keysched_length = Count.apply Q.prove
-(`!Me Mo. LENGTH (toList(expandKeys(Me,Mo))) = 40`,
- SIMP_TAC std_ss [expandKeys_def, toList_def]
-  THEN REPEAT GEN_TAC
-  THEN EVAL_TAC);
-
+val keysched_length = Count.apply Q.prove(
+  `!Me Mo. LENGTH (toList(expandKeys(Me,Mo))) = 40`,
+  SRW_TAC [] [expandKeys_def, toList_def] THEN EVAL_TAC);
 
 (*---------------------------------------------------------------------------*)
 (* The Key-dependent S-boxes *)
 (*---------------------------------------------------------------------------*)
 
-val fun_g_def = Define `
+val fun_g_def = Define`
   fun_g(x, SS) = toLarge(fun_h(x,SS))`;
-
 
 (*---------------------------------------------------------------------------*)
 (* The function FF is a key-dependent permutation on 64-bit values *)
 (*---------------------------------------------------------------------------*)
 
-val FF_def = Define `
+val FF_def = Define`
   FF((R0,R1),(K0,K1),SS) =
   let T0 = fun_g(fromLarge(R0),SS) in
-  let T1 = fun_g(fromLarge(R1 <<<< 8),SS) in
-  let F0 = word32$bitwise_and (T0 + T1 + K0) 0xffffffffw in
-  let F1 = word32$bitwise_and (T0 + 2w*T1+ K1) 0xffffffffw
+  let T1 = fun_g(fromLarge(R1 #<< 8),SS) in
+  let F0 = (T0 + T1 + K0) && 0xffffffffw in
+  let F1 = (T0 + 2w*T1+ K1) && 0xffffffffw
   in (F0,F1)`;
 
-(*----------------------------------------------------------------------------------*)
-(*-------------Forward round used by the encrypting function------------------------*)
-(*----------------------------------------------------------------------------------*)
+(*---------------------------------------------------------------------------*)
+(*-------------Forward round used by the encrypting function-----------------*)
+(*---------------------------------------------------------------------------*)
 
 (* The operation in each of the 16 rounds *)
-val Round_Op_def = Define `
+
+val Round_Op_def = Define`
   Round_Op((R0,R1,R2,R3),k,ss) =
   let (F0, F1) = FF((R0,R1),GETKEYS(k), ss) in
-  let R0' = (R2 ### F0) >>>> 1 in
-  let R1' = (R3 <<<< 1) ### F1
+  let R0' = (R2 ?? F0) #>> 1 in
+  let R1' = (R3 #<< 1) ?? F1
   in (R0', R1', R0, R1)`;
 
-val  (en_rnd_def, en_rnd_ind)  = Defn.tprove (
+val (en_rnd_def, en_rnd_ind) = Defn.tprove (
     Hol_defn "en_rnd"
     `en_rnd i (b:block) k ss =
      if i=0 then b
      else en_rnd (i-1) (Round_Op(b,k,ss)) (ROTKEYS(k)) ss`,
-  WF_REL_TAC `measure FST`);
+  WF_REL_TAC `measure FST` THEN REPEAT PairRules.PGEN_TAC THEN DECIDE_TAC);
 
 val _ = save_thm ("en_rnd_def", en_rnd_def);
 val _ = save_thm ("en_rnd_ind", en_rnd_ind);
 
-val  fwd_def = Define `
-   fwd(b,k,s) = en_rnd 16 b k s`;
+val fwd_def = Define `fwd(b,k,s) = en_rnd 16 b k s`;
 
-(*----------------------------------------------------------------------------------*)
-(*-------------Backward round used by the decrypting function------------------------*)
-(*----------------------------------------------------------------------------------*)
+(*---------------------------------------------------------------------------*)
+(*-------------Backward round used by the decrypting function----------------*)
+(*---------------------------------------------------------------------------*)
 
 (* Decryption. Note that (R2,R3) at round r+1 = (R0,R1) at round r *)
-val InvRound_Op_def = Define `
+val InvRound_Op_def = Define`
   InvRound_Op((R0,R1,R2,R3),k,ss) =
   let (F0, F1) = FF((R2,R3),GETKEYS(k),ss) in
-  let R0' = (R0 <<<< 1) ### F0 in
-  let R1' = (R1 ### F1) >>>> 1
+  let R0' = (R0 #<< 1) ?? F0 in
+  let R1' = (R1 ?? F1) #>> 1
   in (R2, R3, R0', R1')`;
                       
-val  (de_rnd_def, de_rnd_ind)  = Defn.tprove (
+val (de_rnd_def, de_rnd_ind) = Defn.tprove (
     Hol_defn "de_rnd"
     `de_rnd i (b:block) k ss =
      if i=0 then b
      else InvRound_Op(de_rnd (i-1) b (ROTKEYS(k)) ss, k, ss)`,
-  WF_REL_TAC `measure FST`);
+  WF_REL_TAC `measure FST` THEN REPEAT PairRules.PGEN_TAC THEN DECIDE_TAC);
 
 val _ = save_thm ("en_rnd_def", en_rnd_def);
 val _ = save_thm ("de_rnd__ind", de_rnd_ind);
 
-val  bwd_def = Define `
-   bwd(b,k,s) = de_rnd 16 b k s`;
+val bwd_def = Define `bwd(b,k,s) = de_rnd 16 b k s`;
 
-(* ------------------------------------------------------------------------------*)
-(*-------------Forward and backward round operation inversion lemmas-------------*)
-(*-------------------------------------------------------------------------------*)
+(* --------------------------------------------------------------------------*)
+(*-------------Forward and backward round operation inversion lemmas---------*)
+(*---------------------------------------------------------------------------*)
 
-val Round_Inversion = Q.store_thm
-  ("Round_Inversion",
+val PBETA_ss = simpLib.conv_ss
+  {name="PBETA",trace = 3,conv=K (K PairRules.PBETA_CONV),
+   key = SOME([],``(\(x:'a,y:'b). s1) s2:'c``)};
+
+val Round_Inversion = Q.store_thm("Round_Inversion",
   `!b k s. InvRound_Op(Round_Op(b,k,s),k,s) = b`,
-  SIMP_TAC std_ss [FORALL_BLOCK, FORALL_KEY] THEN RW_TAC std_ss [Round_Op_def] THEN
-  RW_TAC std_ss [InvRound_Op_def] THEN Q.UNABBREV_TAC `R0'` THEN Q.UNABBREV_TAC `R1'` 
-  THEN `1 < WL` by ARW_TAC [WL_def, HB_def] THEN
-  METIS_TAC [WORD_EOR_ASSOC, WORD_EOR_INV, WORD_EOR_ID, Word32_SHIFT_Inversion]
- );
+  SIMP_TAC std_ss [FORALL_BLOCK, FORALL_KEY]
+    THEN SRW_TAC [boolSimps.LET_ss,PBETA_ss] [Round_Op_def,InvRound_Op_def]);
  
 val [Round_Op] = decls "Round_Op";
 val [InvRound_Op] = decls "InvRound_Op";
 
-val Round_Inversion_LEMMA = Q.store_thm
-("Round_Inversion_LEMMA",
- `!b k s. bwd(fwd(b,k,s),k,s) = b`,
-   SIMP_TAC std_ss [FORALL_BLOCK] THEN RESTR_EVAL_TAC [Round_Op, InvRound_Op] THEN
-   RW_TAC std_ss [Round_Inversion]);
-                                                                                                                                               
+val Round_Inversion_LEMMA = Q.store_thm("Round_Inversion_LEMMA",
+  `!b k s. bwd(fwd(b,k,s),k,s) = b`,
+  SIMP_TAC std_ss [FORALL_BLOCK]
+    THEN computeLib.RESTR_EVAL_TAC [Round_Op, InvRound_Op]
+    THEN RW_TAC std_ss [Round_Inversion]);
+
 (*---------------------------------------------------------------------------*)
 (* Input whitening and output whitening                                      *)
 (*---------------------------------------------------------------------------*)
 
-val In_Whiten_def = Define `
+val In_Whiten_def = Define`
   In_Whiten(b:block, k) =
     let (R0,R1,R2,R3) = b in
-    (R0 ### FST(GETKEYS(k)), R1 ### SND(GETKEYS(k)),
-     R2 ### FST(GETKEYS(ROTKEYS(k))), R3 ### SND(GETKEYS(ROTKEYS(k))))`;
+    (R0 ?? FST(GETKEYS(k)), R1 ?? SND(GETKEYS(k)),
+     R2 ?? FST(GETKEYS(ROTKEYS(k))), R3 ?? SND(GETKEYS(ROTKEYS(k))))`;
 
-val Out_Whiten_def = Define `
+val Out_Whiten_def = Define`
   Out_Whiten(b:block, k) =
     let (R0,R1,R2,R3) = b in
-    (R0 ### FST(GETKEYS(ROTKEYS(ROTKEYS(k)))), R1 ### SND(GETKEYS(ROTKEYS(ROTKEYS(k)))),
-     R2 ### FST(GETKEYS(ROTKEYS(ROTKEYS(ROTKEYS(k))))), R3 ### SND(GETKEYS(ROTKEYS(ROTKEYS(ROTKEYS(k))))))`;
+    (R0 ?? FST(GETKEYS(ROTKEYS(ROTKEYS(k)))),
+     R1 ?? SND(GETKEYS(ROTKEYS(ROTKEYS(k)))),
+     R2 ?? FST(GETKEYS(ROTKEYS(ROTKEYS(ROTKEYS(k))))),
+     R3 ?? SND(GETKEYS(ROTKEYS(ROTKEYS(ROTKEYS(k))))))`;
 
-val WHITENING_LEMMA = Q.store_thm
-("WHITENING_LEMMA",
- `!(b:block) (k:keysched).
-  (Out_Whiten(Out_Whiten(b,k),k) = b) /\ (In_Whiten(In_Whiten(b,k),k) = b)`,
-  RW_TAC std_ss [Out_Whiten_def, In_Whiten_def] THEN
-  METIS_TAC [WORD_EOR_ASSOC, WORD_EOR_INV, WORD_EOR_ID]);
+val WHITENING_LEMMA = Q.store_thm("WHITENING_LEMMA",
+  `!(b:block) (k:keysched).
+    (Out_Whiten(Out_Whiten(b,k),k) = b) /\ (In_Whiten(In_Whiten(b,k),k) = b)`,
+  SRW_TAC [] [Out_Whiten_def, In_Whiten_def]);
 
 (*---------------------------------------------------------------------------*)
 (* Encrypt and Decrypt                                                       *)
@@ -520,12 +509,12 @@ val WHITENING_LEMMA = Q.store_thm
     Finally the output whitening step undoes the `swap' of the
     last round, and xors the data words with 4 words of the expanded key.*)
 
-val TwofishEncrypt_def = Define `
+val TwofishEncrypt_def = Define`
   TwofishEncrypt initM b =
   let (k, ss) = (expandKeys(genM(initM)), genS(initM))
   in  Out_Whiten(fwd(In_Whiten(b,k),ROTKEYS8(k),ss), k)`;
 
-val TwofishDecrypt_def = Define `
+val TwofishDecrypt_def = Define`
   TwofishDecrypt initM b =
   let (k, ss) = (expandKeys(genM(initM)), genS(initM))
   in  In_Whiten(bwd(Out_Whiten(b,k),ROTKEYS8(k),ss), k)`;
@@ -534,27 +523,26 @@ val TwofishDecrypt_def = Define `
 (* Main Lemma				                                     *)
 (*---------------------------------------------------------------------------*)
 
-val TWOFISH_LEMMA = Q.store_thm
-("TWOFISH_LEMMA",
- `!(plaintext:block) (keys:initkeys).
+val TWOFISH_LEMMA = Q.store_thm("TWOFISH_LEMMA",
+  `!(plaintext:block) (keys:initkeys).
      TwofishDecrypt keys (TwofishEncrypt keys plaintext) = plaintext`,
-   RW_TAC std_ss [TwofishEncrypt_def] THEN RW_TAC std_ss [TwofishDecrypt_def] THEN
-   RW_TAC std_ss [WHITENING_LEMMA, Round_Inversion_LEMMA]);
+  RW_TAC std_ss [TwofishEncrypt_def]
+    THEN RW_TAC std_ss [TwofishDecrypt_def]
+    THEN RW_TAC std_ss [WHITENING_LEMMA, Round_Inversion_LEMMA]);
 
 (*---------------------------------------------------------------------------*)
 (* Basic theorem about encryption/decryption                                 *)
 (*---------------------------------------------------------------------------*)
 
-val TWOFISH_def = Define
- `TWOFISH (keys) = 
+val TWOFISH_def = Define`
+  TWOFISH (keys) = 
   (TwofishEncrypt keys,  TwofishDecrypt keys)`;
-                                                                                                
-val TWOFISH_CORRECT = Q.store_thm
-  ("TWOFISH_CORRECT",
+
+val TWOFISH_CORRECT = Q.store_thm("TWOFISH_CORRECT",
    `!key plaintext.
        ((encrypt,decrypt) = TWOFISH key)
        ==>
        (decrypt (encrypt plaintext) = plaintext)`,
          RW_TAC std_ss [TWOFISH_def,LET_THM,TWOFISH_LEMMA]);
-                                                                                                         
+
 val _ = export_theory();
